proved that iter respects the trace refinement relation and found a counterexample to the proposition that bind is monotonic for itree_spec wrt spec refinement

theories/Dijkstra/EuttEv.v
@@ -134,3 +134,98 @@ Proof.
     + pclearbot. constructor. pstep_reverse.
     + constructor. eapply IHeuttEvF; eauto.
 Qed.
+
+
+Section eqitC_euttEv.
+  Context {E1 E2 : Type -> Type} {R1 R2 : Type} (RR : R1 -> R2 -> Prop).
+  (* Question, is it a problem that I don't have the booleans, is that necessary? 
+     Would be simple to add but would necessitate some busy work *)
+
+  (* A transitivity functor *)
+  Variant eqit_trans_clo  (b1 b2 b1' b2' : bool)  (r : itree E1 R1 -> itree E2 R2 -> Prop) : 
+    itree E1 R1 -> itree E2 R2 -> Prop := 
+    eqit_trans_clo_intro t1 t2 t1' t2' RR1 RR2
+      (EQVl: eqit RR1 b1 b1' t1 t1')
+      (EQVr: eqit RR2 b2 b2' t2 t2')
+      (REL: r t1' t2')
+      (LERR1: forall x x' y, RR1 x x' -> RR x' y -> RR x y)
+      (LERR2: forall x y y', RR2 y y' -> RR x y' -> RR x y) :
+      eqit_trans_clo b1 b2 b1' b2' r t1 t2.
+  Hint Constructors eqit_trans_clo : core.
+  (* sets directionality *)
+  Definition eqitC_euttEv b1 b2 := eqit_trans_clo b1 b2 false false.
+  Hint Unfold eqitC_euttEv : core.
+
+  Lemma eqitC_euttEv_mon b1 b2 r1 r2 t1 t2 
+    (IN : eqitC_euttEv b1 b2 r1 t1 t2)
+    (LE : r1 <2= r2) :
+    eqitC_euttEv b1 b2 r2 t1 t2.
+  Proof.
+    destruct IN; econstructor; eauto.
+  Qed.
+
+  Hint Resolve eqitC_euttEv_mon : paco.
+    
+
+End eqitC_euttEv.
+
+(*replicate this proof for the models functor*)
+Lemma eqitC_euttEv_wcompat (b1 b2 : bool) E1 E2 R1 R2 (REv : forall A B, E1 A -> E2 B -> Prop) 
+      (RAns : forall A B, E1 A -> A -> E2 B -> B -> Prop ) (RR : R1 -> R2 -> Prop) 
+     (vclo: (itree E1 R1 -> itree E2 R2 -> Prop) -> (itree E1 R1 -> itree E2 R2 -> Prop) )
+     (MON: monotone2 vclo)
+      (CMP: compose (eqitC_euttEv RR b1 b2) vclo <3= compose vclo (eqitC_euttEv RR b1 b2)) :
+  wcompatible2 (EuttEv.euttEv_ REv RAns RR vclo) (eqitC_euttEv RR b1 b2).
+Proof.
+  constructor; eauto with paco.
+  { red. intros. eapply eqitC_euttEv_mon; eauto. }
+  intros.
+  dependent destruction PR. punfold EQVl. punfold EQVr. unfold_eqit.
+  hinduction REL before r; intros; clear t1' t2'.
+  - remember (RetF r1) as x. red.
+    hinduction EQVl before r; intros; subst; try inv Heqx; eauto; (try constructor; eauto).
+    remember (RetF r3) as x. hinduction EQVr before r; intros; subst; try inv Heqx; (try constructor; eauto).
+  - red. remember (TauF m1) as x.
+    hinduction EQVl before r; intros; subst; try inv Heqx; try inv CHECK; ( try (constructor; eauto; fail )).
+    remember (TauF m3) as y.
+    hinduction EQVr before r; intros; subst; try inv Heqy; try inv CHECK; (try (constructor; eauto; fail)).
+    pclearbot. constructor. gclo. econstructor; eauto with paco.
+  - remember (TauF t1) as x. red.
+    hinduction EQVl before r; intros; subst; try inv Heqx; try inv CHECK; (try (constructor; eauto; fail)).
+    pclearbot. punfold REL. constructor. eapply IHREL; eauto.
+  - remember (TauF t2) as y. red.
+    hinduction EQVr before r; intros; subst; try inv Heqy; try inv CHECK; (try (constructor; eauto; fail)).
+    pclearbot. punfold REL. constructor. eapply IHREL; eauto.
+  - remember (VisF e1 k1) as x. red.
+    hinduction EQVl before r; intros; subst; try dependent destruction Heqx; try inv CHECK; try (constructor; eauto; fail).
+    remember (VisF e2 k3) as y.
+    hinduction EQVr before r; intros; subst; try dependent destruction Heqy; try inv CHECK; try (constructor; eauto; fail).
+    constructor; auto. intros. apply H0 in H1. pclearbot. eapply MON.
+    + eapply CMP. red. econstructor; eauto.
+    + intros. apply gpaco2_clo; auto.
+Qed.
+
+Definition eqitC_euttEv_wcompat' := eqitC_euttEv_wcompat true true.
+
+Hint Resolve (eqitC_euttEv_wcompat') : paco.
+
+Global Instance geuttEv_cong_eqit {R1 R2 : Type} {E1 E2 : Type -> Type} {REv : forall A B, E1 A -> E2 B -> Prop}
+      {RAns : forall A B, E1 A -> A -> E2 B -> B -> Prop} {RR1 RR2} {RS : R1 -> R2 -> Prop} r rg
+      (LERR1: forall x x' y, (RR1 x x': Prop) -> (RS x' y: Prop) -> RS x y)
+       (LERR2: forall x y y', (RR2 y y': Prop) -> RS x y' -> RS x y) :
+    Proper (eq_itree RR1 ==> eq_itree RR2 ==> flip impl)
+         (gpaco2 (EuttEv.euttEv_ REv RAns RS id) (eqitC_euttEv RS true true) r rg).
+Proof.
+  repeat intro. gclo. econstructor; eauto; 
+  try eapply eqit_mon; try apply H; try apply H0; auto.
+Qed.
+
+Global Instance geuttEv_cong_euttge {R1 R2 : Type} {E1 E2 : Type -> Type} {REv : forall A B, E1 A -> E2 B -> Prop}
+      {RAns : forall A B, E1 A -> A -> E2 B -> B -> Prop} {RR1 RR2} {RS : R1 -> R2 -> Prop} r rg
+      (LERR1: forall x x' y, (RR1 x x': Prop) -> (RS x' y: Prop) -> RS x y)
+       (LERR2: forall x y y', (RR2 y y': Prop) -> RS x y' -> RS x y) :
+    Proper (euttge RR1 ==> euttge RR2 ==> flip impl)
+         (gpaco2 (EuttEv.euttEv_ REv RAns RS id) (eqitC_euttEv RS true true) r rg).
+Proof.
+  repeat intro. gclo. econstructor; eauto.
+Qed.
